refine jump-related part

verilog_src/pipeline/agp32_processor.sv
@@ -19,7 +19,7 @@ module agp32_processor(
 );
 
 logic[2:0] state = 3'd3;
-logic[63:0][31:0]R = '0;
+logic[31:0] R[63:0] = '{0, 0, 0, 0, 0, 0, 0, 0, 0, 0, 0, 0, 0, 0, 0, 0, 0, 0, 0, 0, 0, 0, 0, 0, 0, 0, 0, 0, 0, 0, 0, 0, 0, 0, 0, 0, 0, 0, 0, 0, 0, 0, 0, 0, 0, 0, 0, 0, 0, 0, 0, 0, 0, 0, 0, 0, 0, 0, 0, 0, 0, 0, 0, 0};
 logic[31:0] acc_arg = 'x;
 logic acc_arg_ready = 0;
 logic do_interrupt = 0;
@@ -34,9 +34,8 @@ logic checkA = 'x;
 logic checkB = 'x;
 logic checkW = 'x;
 logic[31:0] IF_PC_input = 'x;
-logic[31:0] IF_instr = 'x;
+logic[31:0] IF_instr = 32'd63;
 logic IF_PC_write_enable = 'x;
-logic[1:0] PC_sel = 2'd0;
 logic[31:0] ID_PC = 'x;
 logic[31:0] ID_instr = 32'd63;
 logic[31:0] ID_read_dataA = 'x;
@@ -91,6 +90,8 @@ logic EX_isAcc = 'x;
 logic EX_NOP_flag = 'x;
 logic EX_compute_enable = 'x;
 logic[1:0] EX_PC_sel = 2'd0;
+logic EX_jump_sel = 0;
+logic[31:0] EX_jump_addr = 'x;
 logic[2:0] EX_ForwardA = 3'd0;
 logic[2:0] EX_ForwardB = 3'd0;
 logic[2:0] EX_ForwardW = 3'd0;
@@ -154,15 +155,7 @@ IF_instr = ready ? inst_rdata : 32'd63;
 end
 
 always_comb begin
-if ((EX_PC_sel == 2'd1) || (((EX_PC_sel == 2'd2) && (EX_ALU_res == 32'd0)) || ((EX_PC_sel == 2'd3) && (!(EX_ALU_res == 32'd0))))) begin
-PC_sel = EX_PC_sel;
-end else begin
-PC_sel = 2'd0;
-end
-end
-
-always_comb begin
-IF_PC_input = (PC_sel == 2'd0) ? (PC + 32'd4) : ((PC_sel == 2'd1) ? EX_ALU_res : ((PC_sel == 2'd2) ? (EX_PC + EX_dataW_updated) : (EX_PC + EX_dataW_updated)));
+IF_PC_input = EX_jump_sel ? EX_jump_addr : (PC + 32'd4);
 end
 
 always_comb begin
@@ -311,6 +304,21 @@ end
 end
 
 always_comb begin
+if (EX_PC_sel == 2'd1) begin
+EX_jump_sel = 1;
+EX_jump_addr = EX_ALU_res;
+end else begin
+if (((EX_PC_sel == 2'd2) && (EX_ALU_res == 32'd0)) || ((EX_PC_sel == 2'd3) && (!(EX_ALU_res == 32'd0)))) begin
+EX_jump_sel = 1;
+EX_jump_addr = EX_PC + EX_dataW_updated;
+end else begin
+EX_jump_sel = 0;
+EX_jump_addr = 32'd0;
+end
+end
+end
+
+always_comb begin
 if ((state == 3'd0) && (!(MEM_opc == 6'd16))) begin
 EX_dataA_rec = EX_dataA_updated;
 EX_dataB_rec = EX_dataB_updated;
@@ -364,7 +372,7 @@ MEM_state_flag = 0;
 MEM_NOP_flag = 0;
 WB_state_flag = 0;
 end else begin
-if ((state == 3'd2) || ((state == 3'd4) || ((state == 3'd6) || (state == 3'd7)))) begin
+if ((state == 3'd2) || ((state == 3'd4) || ((state == 3'd6) || (state == 3'd1)))) begin
 IF_PC_write_enable = 0;
 ID_ID_write_enable = 0;
 ID_flush_flag = 0;
@@ -373,16 +381,6 @@ EX_NOP_flag = 0;
 MEM_state_flag = 0;
 MEM_NOP_flag = 0;
 WB_state_flag = 0;
-end else begin
-if (state == 3'd1) begin
-IF_PC_write_enable = 0;
-ID_ID_write_enable = 0;
-ID_flush_flag = 0;
-ID_EX_write_enable = 0;
-EX_NOP_flag = 0;
-MEM_state_flag = 1;
-MEM_NOP_flag = 0;
-WB_state_flag = 1;
 end else begin
 if (!ready) begin
 IF_PC_write_enable = 0;
@@ -404,7 +402,7 @@ MEM_state_flag = 0;
 MEM_NOP_flag = 1;
 WB_state_flag = 1;
 end else begin
-if (!(PC_sel == 2'd0)) begin
+if (EX_jump_sel) begin
 IF_PC_write_enable = 1;
 ID_ID_write_enable = 0;
 ID_flush_flag = 1;
@@ -422,7 +420,6 @@ EX_NOP_flag = 0;
 MEM_state_flag = 1;
 MEM_NOP_flag = 0;
 WB_state_flag = 1;
-end
 end
 end
 end
@@ -516,28 +513,28 @@ data_out <= WB_isOut ? WB_ALU_res[9:0] : data_out;
 MEM_enable <= 0;
 WB_enable <= 0;
 if (!ready) begin
-state = 3'd7;
+state = 3'd1;
 end else begin
 if (MEM_isInterrupt) begin
-state = 3'd7;
+state = 3'd1;
 command <= 3'd4;
 do_interrupt = 1;
 data_addr <= 32'd0;
 end else begin
 if (MEM_read_mem) begin
-state = 3'd7;
+state = 3'd1;
 command <= 3'd2;
 data_addr <= MEM_dataA;
 end else begin
 if (MEM_write_mem) begin
-state = 3'd7;
+state = 3'd1;
 command <= 3'd3;
 data_addr <= MEM_dataB;
 data_wdata <= MEM_dataA;
 data_wstrb <= 4'd15;
 end else begin
 if (MEM_write_mem_byte) begin
-state = 3'd7;
+state = 3'd1;
 command <= 3'd3;
 data_addr <= MEM_dataB;
 data_wstrb <= 4'd1 << 4'({MEM_dataB[1:0]});
@@ -547,10 +544,6 @@ case (MEM_dataB[1:0])
 2'd2 : data_wdata[23:16] <= MEM_dataA[7:0];
 2'd3 : data_wdata[31:24] <= MEM_dataA[7:0];
 endcase
-end else begin
-if (!(PC_sel == 2'd0)) begin
-state = 3'd1;
-command <= 3'd1;
 end else begin
 if (EX_isAcc) begin
 state = 3'd2;
@@ -564,10 +557,15 @@ end
 end
 end
 end
-end
 3'd1 : begin
 if (ready && (command == 3'd0)) begin
+if (do_interrupt) begin
+state = 3'd4;
+do_interrupt = 0;
+interrupt_req <= 1;
+end else begin
 state = 3'd6;
+end
 end
 command <= 3'd0;
 end
@@ -590,18 +588,6 @@ state = 3'd0;
 command <= 3'd1;
 MEM_enable <= 1;
 WB_enable <= 1;
-end
-3'd7 : begin
-if (ready && (command == 3'd0)) begin
-if (do_interrupt) begin
-state = 3'd4;
-do_interrupt = 0;
-interrupt_req <= 1;
-end else begin
-state = 3'd6;
-end
-end
-command <= 3'd0;
 end
 endcase
 end else begin
